wip (mostly finished young_diagram.lean and ssyt.lean)

src/ssyt.lean
@@ -24,8 +24,16 @@ instance ssyt.to_fun {μ : young_diagram} :
 --   {i1 i2 j : ℕ} (hi : i1 < i2) (hcell : (i2, j) ∈ μ) : T i1 j < T i2 j :=
 --   T.col_strict' hi hcell
 
-lemma ssyt.zeros {μ : young_diagram} (T : ssyt μ) : 
-  ∀ {i j : ℕ}, (i, j) ∉ μ → T i j = 0 := T.zeros'
+lemma ssyt.zeros {μ : young_diagram} (T : ssyt μ) 
+  {i j : ℕ} (not_cell : (i, j) ∉ μ) : T i j = 0 := T.zeros' not_cell
+
+lemma ssyt.row_weak' {μ : young_diagram} (T : ssyt μ) {i j1 j2 : ℕ}
+  (hj : j1 ≤ j2) (cell : (i, j2) ∈ μ) : T i j1 ≤ T i j2 :=
+by {cases eq_or_lt_of_le hj, subst h, exact T.row_weak h cell}
+
+lemma ssyt.col_weak {μ : young_diagram} (T : ssyt μ) {i1 i2 j : ℕ}
+  (hi : i1 ≤ i2) (cell : (i2, j) ∈ μ) : T i1 j ≤ T i2 j :=
+by {cases eq_or_lt_of_le hi, subst h, exact le_of_lt (T.col_strict h cell)}
 
 def ssyt.to_fun_cells {μ : young_diagram} (T : ssyt μ) (cc : μ.cells) : ℕ :=
   T cc.val.1 cc.val.2
@@ -55,13 +63,13 @@ def ssyt_bounded.to_ssyt'_bounded {μ : young_diagram} {m : ℕ}
     λ c c' hi hj, begin
     cases c with c hc, cases c with i1 j1,
     cases c' with c' hc', cases c' with i2 j2,
-    change i1 = i2 at hi, change j1 < j2 at hj, subst i2,
+    dsimp at *, subst i2,
     apply TT.val.row_weak hj hc',
   end,
   λ c c' hi hj, begin
     cases c with c hc, cases c with i1 j1,
     cases c' with c' hc', cases c' with i2 j2,
-    change i1 < i2 at hi, change j1 = j2 at hj, subst j2,
+    dsimp at *, subst j2,
     apply TT.val.col_strict hi hc',
   end⟩
 }
@@ -108,3 +116,179 @@ instance ssyt_bounded.fintype {μ : young_diagram} {m : ℕ} :
   fintype.of_equiv _ (ssyt.bounded_equiv μ m).symm
 
 end ssyt_bounded
+
+section legal_replace_add
+
+structure ssyt.legal {μ : young_diagram} (T : ssyt μ) :=
+  (i j val : ℕ)
+  (cell_left : ∀ {j'}, j' < j → (i, j') ∈ μ)
+  (cell_up : ∀ {i'}, i' < i → (i', j) ∈ μ)
+  (left : ∀ {j'}, j' < j → T i j' ≤ val)
+  (up : ∀ {i'}, i' < i → T i' j < val)
+  (right : ∀ {j'}, j < j' → (i, j') ∈ μ → val ≤ T i j')  
+  (down : ∀ {i'}, i < i' → (i', j) ∈ μ → val < T i' j)
+
+def ssyt.legal.replace {μ : young_diagram} {T : ssyt μ}
+  (h : T.legal) (cell : (h.i, h.j) ∈ μ) : ssyt μ :=
+{ entry := λ i j, ite ((i, j) = (h.i, h.j)) h.val (T i j),
+  row_weak := λ i j1 j2 hj cell, begin
+    split_ifs,
+    { refl },
+    { cases h_1, apply h.right hj cell, },
+    { cases h_2, apply h.left hj, },
+    { exact T.row_weak hj cell }
+  end,
+  col_strict := λ i1 i2 j hi cell, begin
+    split_ifs,
+    { cases h_1, cases h_2, exact false.rec _ ((lt_self_iff_false _).mp hi) },
+    { cases h_1, apply h.down hi cell },
+    { cases h_2, apply h.up hi },
+    { exact T.col_strict hi cell }
+  end,
+  zeros' := λ i j not_cell, begin
+    rw [if_neg, T.zeros not_cell],
+    exact λ h_eq, (h_eq ▸ not_cell) cell,
+  end,
+}
+
+def ssyt.legal.to_outer {μ : young_diagram} {T : ssyt μ}
+  (h : T.legal) (not_cell : (h.i, h.j) ∉ μ):
+  μ.outer_corner :=
+{ i := h.i,
+  j := h.j,
+  not_cell := not_cell,
+  cell_left := h.cell_left,
+  cell_up := h.cell_up }
+
+def ssyt.legal.add {μ : young_diagram} {T : ssyt μ}
+  (h : T.legal) (not_cell : (h.i, h.j) ∉ μ) : ssyt (h.to_outer not_cell).add :=
+{ entry := λ i j, ite ((i, j) = (h.i, h.j)) h.val (T i j),
+  row_weak := λ i j1 j2 hj cell, begin
+    rw young_diagram.outer_corner.mem_add at cell,
+    split_ifs,
+    { refl },
+    { cases h_1, cases cell, exact false.rec _ (h_2 cell),
+      apply h.right hj cell },
+    { cases h_2, apply h.left hj },
+    { cases cell, exact false.rec _ (h_2 cell),
+      exact T.row_weak hj cell }
+  end,
+  col_strict := λ i1 i2 j hi cell, begin
+    rw young_diagram.outer_corner.mem_add at cell,
+    split_ifs,
+    { rw prod.mk.inj_iff at h_1, rw prod.mk.inj_iff at h_2,
+      rw [h_1.1, h_2.1, lt_self_iff_false] at hi,
+      exact false.rec _ hi },
+    { cases h_1, cases cell, exact false.rec _ (h_2 cell),
+      apply h.down hi cell },
+    { cases h_2, apply h.up hi },
+    { cases cell, exact false.rec _ (h_2 cell),
+      exact T.col_strict hi cell }
+  end,
+  zeros' := λ i j not_cell, begin
+    rw young_diagram.outer_corner.mem_add at not_cell, push_neg at not_cell,
+    rw [if_neg, T.zeros not_cell.2], exact not_cell.1,
+  end,
+}
+
+lemma ssyt.legal.entry_replace {μ : young_diagram} {T : ssyt μ}
+  (h : T.legal) (cell : (h.i, h.j) ∈ μ) (i j : ℕ) :
+  (h.replace cell) i j = ite ((i, j) = (h.i, h.j)) h.val (T i j) := rfl
+
+lemma ssyt.legal.entry_add {μ : young_diagram} {T : ssyt μ}
+  (h : T.legal) (not_cell : (h.i, h.j) ∉ μ) (i j : ℕ) :
+  (h.add not_cell) i j = ite ((i, j) = (h.i, h.j)) h.val (T i j) := rfl
+
+end legal_replace_add
+
+section weight
+
+def ssyt.strip {μ : young_diagram} (T : ssyt μ) (val : ℕ) : finset (ℕ × ℕ) :=
+  μ.cells.filter (λ c, T c.fst c.snd = val)
+@[simp] lemma ssyt.mem_strip {μ : young_diagram} (T : ssyt μ) {val i j : ℕ} :
+  (i, j) ∈ T.strip val ↔ (i, j) ∈ μ ∧ T i j = val :=
+by { rw [ssyt.strip, finset.mem_filter], refl }
+
+def ssyt.wt {μ : young_diagram} (T : ssyt μ) (val : ℕ) : ℕ :=
+  (T.strip val).card
+
+lemma ssyt.strip_add {μ : young_diagram} (T : ssyt μ) (val : ℕ)
+  (h : T.legal) (not_cell : (h.i, h.j) ∉ μ) :
+  (h.add not_cell).strip val =
+  ite (val = h.val) (insert (h.i, h.j) (T.strip val)) (T.strip val) :=
+begin
+  ext ⟨i, j⟩,
+  rw [ssyt.mem_strip, young_diagram.outer_corner.mem_add, ssyt.legal.entry_add],
+  split_ifs; try {rw finset.mem_insert}; rw ssyt.mem_strip,
+  { cases h_1, cases h_2, 
+    simp only [not_cell, or_false, eq_self_iff_true, and_true, false_and, iff_true],
+    refl, },
+  { cases h_1, simp only [not_cell, ne.symm h_2, and_false, false_and] },
+  { cases h_2, rw [or_iff_right, or_iff_right]; exact h_1 },
+  { rw or_iff_right, exact h_1, }
+end
+
+lemma ssyt.wt_add {μ : young_diagram} (T : ssyt μ) (val : ℕ)
+  (h : T.legal) (not_cell : (h.i, h.j) ∉ μ) :
+  (h.add not_cell).wt val = T.wt val + ite (val = h.val) 1 0 :=
+begin
+  rw [ssyt.wt, ssyt.wt, ssyt.strip_add, apply_ite finset.card],
+  split_ifs,
+  { rw finset.card_insert_of_not_mem,
+    rw ssyt.mem_strip,
+    simp only [not_cell, false_and, not_false_iff] },
+  { rw add_zero }
+end
+
+lemma ssyt.strip_replace {μ : young_diagram} (T : ssyt μ) (val : ℕ)
+  (h : T.legal) (cell : (h.i, h.j) ∈ μ) :
+  ite (val = T h.i h.j) 
+    (insert (h.i, h.j) ((h.replace cell).strip val))
+    ((h.replace cell).strip val) =
+  ite (val = h.val) 
+    (insert (h.i, h.j) (T.strip val)) 
+    (T.strip val) :=
+begin
+  ext ⟨i, j⟩,
+  split_ifs,
+  all_goals {
+    try { rw finset.mem_insert }, try { rw finset.mem_insert },
+    rw [ssyt.mem_strip, ssyt.mem_strip, h.entry_replace],
+  },
+  { split_ifs, cases h_3,
+    simp only [eq_self_iff_true, true_or],
+    simp only [h_3] },
+  { split_ifs, cases h_3,
+    simp only [eq_self_iff_true, true_or, true_iff], exact ⟨cell, h_1.symm⟩,
+    rw or_iff_right h_3 },
+  { cases h_2, split_ifs, cases h_3, 
+    simp only [eq_self_iff_true, and_true, true_or, iff_true], exact cell,
+    rw or_iff_right h_3 },
+  { rw and.congr_right_iff, intro hij,
+    split_ifs, cases h_3, simp only [ne.symm h_1, ne.symm h_2], refl },
+end
+
+-- new strip of k's + (box if T h.i h.j = k) = 
+-- (old strip of k's) + (box if h.val = k)
+
+def ssyt.wt_replace {μ : young_diagram} (T : ssyt μ) (val : ℕ)
+  (h : T.legal) (cell : (h.i, h.j) ∈ μ) :
+  (h.replace cell).wt val + ite (val = T h.i h.j) 1 0 =
+  T.wt val + ite (val = h.val) 1 0 :=
+begin
+  have key := T.strip_replace val h cell,
+  rw [ssyt.wt, ssyt.wt],
+  split_ifs; split_ifs at key,
+  { rw [finset.insert_eq_of_mem, finset.insert_eq_of_mem] at key, rw key,
+    rw ssyt.mem_strip, exact ⟨cell, h_1.symm⟩,
+    rw [ssyt.mem_strip, h.entry_replace, if_pos rfl], exact ⟨cell, h_2.symm⟩ },
+  { rw [add_zero, ← key, finset.card_insert_of_not_mem],
+    rw [ssyt.mem_strip, ssyt.legal.entry_replace, if_pos rfl],
+    exact λ h, ne.symm h_2 h.2 },
+  { rw [key, add_zero, finset.card_insert_of_not_mem],
+    rw ssyt.mem_strip,
+    exact λ h, ne.symm h_1 h.2 },
+  { rw [key, add_zero] },
+end
+
+end weight
