src/young_diagram.lean
@@ -6,17 +6,19 @@ section young_diagram
 @[ext]
 structure young_diagram :=
   (cells : finset (ℕ × ℕ))
-  (nw_of' : ∀ {i1 i2 j1 j2}, 
+  (nw_of' : ∀ {i1 i2 j1 j2 : ℕ}, 
     i1 ≤ i2 → j1 ≤ j2 → (i2, j2) ∈ cells → (i1, j1) ∈ cells)
 
 instance young_diagram.has_mem : has_mem (ℕ × ℕ) young_diagram :=
 { mem := λ c μ, c ∈ μ.cells, }
+
+lemma young_diagram.mem_cells (μ : young_diagram) (c : ℕ × ℕ) :
+  c ∈ μ.cells ↔ c ∈ μ := iff.rfl
+
 def young_diagram.nw_of (μ : young_diagram) 
   {i1 i2 j1 j2 : ℕ} (hi : i1 ≤ i2) (hj : j1 ≤ j2) (hcell : (i2, j2) ∈ μ) : 
   (i1, j1) ∈ μ := μ.nw_of' hi hj hcell
--- def young_diagram.nw_of_c (μ : young_diagram) {c c' : ℕ × ℕ} 
---   (hi : c.fst ≤ c'.fst) (hj : c.snd ≤ c'.snd) (hcell : c' ∈ μ) : c ∈ μ :=
--- by { cases c, cases c', apply μ.nw_of hi hj hcell, }
+
 instance young_diagram.has_subset : has_subset young_diagram :=
 { subset := λ μ ν, μ.cells ⊆ ν.cells }
 instance young_diagram.has_emptyc : has_emptyc young_diagram :=
@@ -24,149 +26,105 @@ instance young_diagram.has_emptyc : has_emptyc young_diagram :=
 
 def μ_empty := (∅ : young_diagram)
 
+def young_diagram.size (μ : young_diagram) := μ.cells.card
 def young_diagram.row (μ : young_diagram) (i : ℕ) := μ.cells.filter (λ c, c.fst = i)
 def young_diagram.col (μ : young_diagram) (j : ℕ) := μ.cells.filter (λ c, c.snd = j)
-def young_diagram.row_len (μ : young_diagram) (i : ℕ) := (μ.row i).card
-def young_diagram.col_len (μ : young_diagram) (j : ℕ) := (μ.col j).card
-def young_diagram.size (μ : young_diagram) := μ.cells.card
+
+lemma young_diagram.row_def (μ : young_diagram) {i : ℕ} :
+  μ.row i = μ.cells.filter (λ c, c.fst = i) := rfl
+lemma young_diagram.col_def (μ : young_diagram) {j : ℕ} :
+  μ.col j = μ.cells.filter (λ c, c.snd = j) := rfl
+
+lemma young_diagram.mem_row_iff (μ : young_diagram) {i : ℕ} (c : ℕ × ℕ) :
+  c ∈ μ.row i ↔ c ∈ μ ∧ c.fst = i :=
+by {rw [young_diagram.row_def, finset.mem_filter], refl}
+lemma young_diagram.mem_col_iff (μ : young_diagram) {j : ℕ} (c : ℕ × ℕ) :
+  c ∈ μ.col j ↔ c ∈ μ ∧ c.snd = j :=
+by {rw [young_diagram.col_def, finset.mem_filter], refl}
+
+lemma young_diagram.mem_iff_mem_row (μ : young_diagram) {i j : ℕ} :
+  (i, j) ∈ μ ↔ (i, j) ∈ μ.row i :=
+by rw [young_diagram.mem_row_iff, and_iff_left rfl]
+lemma young_diagram.mem_iff_mem_col (μ : young_diagram) {i j : ℕ} :
+  (i, j) ∈ μ ↔ (i, j) ∈ μ.col j :=
+by rw [young_diagram.mem_col_iff, and_iff_left rfl]
+
+lemma young_diagram.row_len_aux (μ : young_diagram) (i : ℕ) : ∃ j, (i, j) ∉ μ := 
+begin
+  obtain ⟨j, hj⟩ := infinite.exists_not_mem_finset ((μ.row i).image prod.snd), 
+  use j, intro hij, apply hj,
+  rw finset.mem_image, rw μ.mem_iff_mem_row at hij,
+  exact ⟨_, hij, rfl⟩,
+end
+lemma young_diagram.col_len_aux (μ : young_diagram) (j : ℕ) : ∃ i, (i, j) ∉ μ := 
+begin
+  obtain ⟨i, hi⟩ := infinite.exists_not_mem_finset ((μ.col j).image prod.fst), 
+  use i, intro hij, apply hi,
+  rw finset.mem_image, rw μ.mem_iff_mem_col at hij,
+  exact ⟨_, hij, rfl⟩,
+end
+
+def young_diagram.row_len (μ : young_diagram) (i : ℕ) : ℕ := 
+  nat.find (μ.row_len_aux i)
+def young_diagram.col_len (μ : young_diagram) (j : ℕ) : ℕ := 
+  nat.find (μ.col_len_aux j)
 def young_diagram.row_lens (μ : young_diagram) : list ℕ := 
   list.map μ.row_len (list.range (μ.col_len 0))
 def young_diagram.col_lens (μ : young_diagram) : list ℕ := 
   list.map μ.col_len (list.range (μ.row_len 0))
 
-lemma young_diagram.row_def (μ : young_diagram) {i : ℕ} :
-  μ.row i = μ.cells.filter (λ c, c.fst = i) := rfl
+lemma young_diagram.row_len_def (μ : young_diagram) {i : ℕ} :
+  μ.row_len i = nat.find (μ.row_len_aux i) := rfl
+lemma young_diagram.col_len_def (μ : young_diagram) {j : ℕ} :
+  μ.col_len j = nat.find (μ.col_len_aux j) := rfl
 
-lemma young_diagram.mem_row_iff (μ : young_diagram) {i : ℕ} (c : ℕ × ℕ) :
-  c ∈ μ.row i ↔ c ∈ μ ∧ c.fst = i :=
-begin
-  rw [young_diagram.row_def, finset.mem_filter], refl,
-end
-
-lemma young_diagram.row_def' (μ : young_diagram) (i : ℕ) : 
-  μ.row i = finset.product {i} (finset.range (μ.row_len i)) :=
-begin
-  by_cases (μ.row i).nonempty, rotate,
-  { rw finset.not_nonempty_iff_eq_empty at h,
-    rw [young_diagram.row_len, h, 
-      finset.card_empty, finset.range_zero, finset.product_empty], },
-
-  have key : ∀ b : ℕ, (i, b) ∈ μ → 
-    finset.product {i} (finset.range b.succ) ⊆ μ.row i,
-  { rintros b hb ⟨i', j'⟩ h',
-    rw [finset.mem_product, finset.mem_singleton, finset.mem_range] at h',
-    change i' = _ ∧ j' < _ at h', obtain ⟨hi, hj⟩ := h', subst i',
-    rw young_diagram.mem_row_iff,
-    exact ⟨μ.nw_of (le_refl i) (nat.lt_succ_iff.mp hj) hb, rfl⟩, },
-  
-  { have key' : ∀ j, j ∈ (μ.row i).image prod.snd ↔ (i, j) ∈ μ,
-    { intro j, rw finset.mem_image,
-      split, rintro ⟨⟨a, b⟩, h, h'⟩,
-      rw young_diagram.mem_row_iff at h, obtain ⟨hj', _ : a = i⟩ := h, subst a,
-      change b = _ at h', subst b, exact hj',
-      intro h, use (i, j), rw young_diagram.mem_row_iff,
-      exact ⟨⟨h, rfl⟩, rfl⟩, },
-
-    set j := ((μ.row i).image prod.snd).max' (h.image _) with hj,
-
-    have : μ.row i = finset.product {i} (finset.range j.succ),
-    { apply subset_antisymm,
-      rotate, apply key, rw ← key', apply finset.max'_mem,
-      rintro ⟨a, b⟩ hab,
-      rw young_diagram.mem_row_iff at hab, 
-      obtain ⟨hab, _ : a = i⟩ := hab, subst a,
-      rw [finset.mem_product, finset.mem_singleton, finset.mem_range],
-      split, refl, rw nat.lt_succ_iff, 
-      apply finset.le_max', rw key', exact hab, },
-    
-    rw this, congr, rw young_diagram.row_len, rw this,
-    rw [finset.card_product, finset.card_singleton, one_mul, finset.card_range],
-  },
-end
-
-lemma young_diagram.mem_row_iff' (μ : young_diagram) (i j : ℕ) :
+lemma young_diagram.mem_row_iff' (μ : young_diagram) {i j : ℕ} :
   (i, j) ∈ μ ↔ j < μ.row_len i :=
 begin
-  rw (_ : (i, j) ∈ μ ↔ (i, j) ∈ μ.row i),
-  rw young_diagram.row_def',
-  rw [finset.mem_product, finset.mem_singleton, finset.mem_range],
-  rw and_iff_right, refl,
-  rw [young_diagram.row_def, finset.mem_filter, and_iff_left rfl], refl,
+  rw [μ.row_len_def, nat.lt_find_iff], push_neg,
+  split; intro h,
+  exact λ m hmj, μ.nw_of (le_refl i) hmj h,
+  exact h _ (le_refl _),
+end
+lemma young_diagram.mem_col_iff' (μ : young_diagram) {i j : ℕ} :
+  (i, j) ∈ μ ↔ i < μ.col_len j :=
+begin
+  rw [μ.col_len_def, nat.lt_find_iff], push_neg,
+  split; intro h,
+  exact λ m hmj, μ.nw_of hmj (le_refl j) h,
+  exact h _ (le_refl _),
 end
 
--- lemma young_diagram.row_not_cell (μ : young_diagram) (i : ℕ) : (i, μ.row_len i) ∉ μ :=
--- begin
---   by_contra, apply @nat.not_succ_le_self (μ.row_len i),
---   suffices : finset.product {i} (finset.range (μ.row_len i).succ) ⊆ μ.row i,
---     convert finset.card_le_of_subset this,
---     rw [finset.card_product, finset.card_singleton, one_mul, finset.card_range],
---   rintros ⟨a, b⟩ hab, 
---   rw [finset.mem_product, finset.mem_singleton, finset.mem_range,
---       nat.lt_succ_iff] at hab,
---   change a = _ ∧ b ≤ _ at hab, obtain ⟨ha, hb⟩ := hab, subst a,
---   rw [young_diagram.row_def, finset.mem_filter],
---   exact ⟨μ.nw_of (le_refl _) hb h, rfl⟩,
--- end
+lemma young_diagram.row_eq_prod_range (μ : young_diagram) {i : ℕ} :
+  μ.row i = finset.product {i} (finset.range (μ.row_len i)) :=
+begin
+  ext ⟨a, b⟩,
+  rw [finset.mem_product, finset.mem_singleton, finset.mem_range,
+      μ.mem_row_iff, μ.mem_row_iff',
+      and_comm, and.congr_right_iff],
+  rintro rfl, refl,
+end
+lemma young_diagram.col_eq_prod_range (μ : young_diagram) {j : ℕ} :
+  μ.col j = finset.product (finset.range (μ.col_len j)) {j} :=
+begin
+  ext ⟨a, b⟩,
+  rw [finset.mem_product, finset.mem_singleton, finset.mem_range,
+      μ.mem_col_iff, μ.mem_col_iff', and.congr_left_iff],
+  rintro rfl, refl,
+end
 
--- lemma young_diagram.cell_of_lt_row_len (μ : young_diagram) (i j : ℕ) :
---   j < μ.row_len i → (i, j) ∈ μ :=
--- begin
---   by_contra, push_neg at h,
---   rw ← lt_self_iff_false (μ.row_len i),
---   suffices : μ.row i ⊂ finset.product {i} (finset.range (μ.row_len i)),
---     convert finset.card_lt_card this,
---     rw [finset.card_product, finset.card_singleton, one_mul, finset.card_range],
---   split,
---   { rintros ⟨a, b⟩ hab,
---     rw [finset.mem_product, finset.mem_singleton, finset.mem_range],
---     rw [young_diagram.row_def, finset.mem_filter] at hab,
---     split, exact hab.2,
---    },
--- end
-
--- lemma young_diagram.mem_row_iff (μ : young_diagram) (c : ℕ × ℕ) :
---   c ∈ μ ↔ c.snd < μ.row_len c.fst :=
--- begin
---   cases c with i j,
---   split; intro h,
---   { by_contra h_le, push_neg at h_le,
---     exact μ.row_not_cell i (μ.nw_of (le_refl _) h_le h), },
---   { 
-
---   },
---   -- rw (_ : c ∈ μ ↔ c ∈ μ.row c.fst),
---   -- rotate, 
---   -- { unfold young_diagram.row, 
---   --   rw [finset.mem_filter, and_iff_left rfl], refl, },
---   -- by_cases h : μ.row c.fst = ∅,
---   -- { unfold young_diagram.row_len, 
---   --   rw [h, finset.card_empty, iff_false_intro (nat.not_lt_zero c.snd)], refl, },
---   -- rw ← finset.not_nonempty_iff_eq_empty at h, push_neg at h,
-  
--- end
--- lemma young_diagram.row_len_def' (μ : young_diagram) {i : ℕ} :
--- lemma young_diagram.row_def' (μ : young_diagram) (i : ℕ) :
---   μ.row i = ({i} : finset ℕ).product (finset.range (μ.row_len i)) :=
--- begin
---   ext ⟨a, b⟩,
---   rw [μ.row_def, finset.mem_filter, finset.mem_product, finset.mem_range,
---       finset.mem_singleton],
---   change ((a, b) ∈ μ ∧ a = i) ↔ (a = i ∧ b < _),
---   split; rintro ⟨h, h'⟩; subst a,
---   split, refl, unfold young_diagram.row_len,
--- end
-
--- lemma young_diagram.mem_row_iff (μ : young_diagram) (c : ℕ × ℕ) :
---   c ∈ μ ↔ c.snd < μ.row_len c.fst :=
--- begin
---   unfold young_diagram.row_len,
---   -- rw (_ : μ.row c.fst = finset.range (μ.row_len c.fst)),
---   rw (_ : c ∈ μ ↔ c ∈ μ.row c.fst),
-
---   sorry,
---   unfold young_diagram.row, 
---   rw [finset.mem_filter, and_iff_left rfl], refl,
--- end
+lemma young_diagram.row_len_eq_card (μ : young_diagram) {i : ℕ} :
+  μ.row_len i = (μ.row i).card :=
+begin
+  rw μ.row_eq_prod_range, 
+  rw [finset.card_product, finset.card_singleton, finset.card_range, one_mul],
+end
+lemma young_diagram.col_len_eq_card (μ : young_diagram) {j: ℕ} :
+  μ.col_len j = (μ.col j).card :=
+begin
+  rw μ.col_eq_prod_range,
+  rw [finset.card_product, finset.card_singleton, finset.card_range, mul_one],
+end
 
 section of_row_lens
 
@@ -196,12 +154,12 @@ lemma list_decr_iff :
 end
 
 @[simp]
-def young_diagram.cells_of_row_lens (w :list ℕ) : finset (ℕ × ℕ) :=
+def young_diagram.cells_of_row_lens (w : list ℕ) : finset (ℕ × ℕ) :=
   finset.bUnion 
     (finset.range w.length)
     (λ i, ({i} : finset ℕ).product (finset.range (w.inth i)))
 
-lemma young_diagram.cells_of_row_lens_mem (w : list ℕ) (c : ℕ × ℕ):
+lemma young_diagram.mem_of_row_lens (w : list ℕ) (c : ℕ × ℕ):
   c ∈ young_diagram.cells_of_row_lens w ↔ c.snd < w.inth c.fst :=
 begin
   unfold young_diagram.cells_of_row_lens,
@@ -222,48 +180,20 @@ begin
              ⟨finset.mem_singleton_self _, finset.mem_range.mpr h⟩⟩, },
 end
 
--- def young_diagram.cells_of_row_lens : list ℕ → finset (ℕ × ℕ)
--- | [] := finset.empty
--- | (x :: xs) := 
---   (({0} : finset ℕ).product (finset.range x)) ∪
---   finset.map
---     (function.embedding.prod_map 
---       ⟨nat.succ, by apply nat.succ.inj⟩
---       (function.embedding.refl ℕ))
---   (young_diagram.cells_of_row_lens xs)
-
--- lemma young_diagram.cells_of_row_lens_mem (w : list ℕ) (c : ℕ × ℕ):
---   c ∈ young_diagram.cells_of_row_lens w ↔ c.snd < w.inth c.fst :=
--- begin 
---   cases w with x xs,
---     exact (false_iff _).mpr (nat.not_lt_zero _),
---   cases c with i j,
---   cases i,
---   { change (0, j) ∈ _ ∪ _ ↔ j < x, 
---     rw finset.mem_union,
-
---   },
-
--- end
--- | [] c := (false_iff _).mpr (nat.not_lt_zero _)
--- | (x :: xs) (0, j) := begin
---   change _ ↔ j < x,
---   split; intro h,
---   { replace h := (finset.mem_union.mp h),
-
---    },
--- end
--- | (x :: xs) (nat.succ i, j) := sorry
-
 def young_diagram.of_row_lens (r : list ℕ) (h : list_decr r) : young_diagram :=
 { cells := young_diagram.cells_of_row_lens r,
   nw_of' := λ i1 i2 j1 j2 hi hj hcell, begin
-    rw young_diagram.cells_of_row_lens_mem at *,
+    rw young_diagram.mem_of_row_lens at *,
     change j1 < r.inth i1, change j2 < r.inth i2 at hcell,
     apply lt_of_le_of_lt hj,
     apply lt_of_lt_of_le hcell,
     apply list_decr_iff.mp h, exact hi,
   end,}
+
+@[simp] lemma young_diagram.of_row_lens.mem (w : list ℕ) (h : list_decr w)
+  {c : ℕ × ℕ} :
+  c ∈ young_diagram.of_row_lens w h ↔ c.snd < w.inth c.fst :=
+young_diagram.mem_of_row_lens w c
 
 end of_row_lens
 
@@ -283,53 +213,211 @@ section corners
 structure young_diagram.inner_corner (μ : young_diagram) :=
   (i j : ℕ)
   (cell : (i, j) ∈ μ)
-  (row_right : ∀ {j'}, j < j' → (i, j') ∉ μ)
-  (col_down : ∀ {i'}, i < i' → (i', j) ∉ μ)
+  (cell_right : ∀ {j'}, j < j' → (i, j') ∉ μ)
+  (cell_down : ∀ {i'}, i < i' → (i', j) ∉ μ)
 
 structure young_diagram.outer_corner (μ : young_diagram) :=
   (i j : ℕ)
   (not_cell : (i, j) ∉ μ)
-  (row_left : ∀ {j'}, j' < j → (i, j') ∈ μ)
-  (col_up : ∀ {i'}, i' < i → (i', j) ∈ μ)
+  (cell_left : ∀ {j'}, j' < j → (i, j') ∈ μ)
+  (cell_up : ∀ {i'}, i' < i → (i', j) ∈ μ)
+
+instance young_diagram.dec_cell_right (μ : young_diagram)
+  (i j : ℕ) : decidable (∀ {j'}, j < j' → (i, j') ∉ μ) :=
+if hj : j.succ < μ.row_len i
+then is_false (λ h', h' (lt_add_one j) (μ.mem_row_iff'.mpr hj))
+else is_true (λ j' h' hcell, hj (μ.mem_row_iff'.mp (μ.nw_of (le_refl _) h' hcell)))
+
+instance young_diagram.dec_cell_down (μ : young_diagram)
+  (i j : ℕ) : decidable (∀ {i'}, i < i' → (i', j) ∉ μ) :=
+if hi : i.succ < μ.col_len j
+then is_false (λ h', h' (lt_add_one i) (μ.mem_col_iff'.mpr hi))
+else is_true (λ j' h' hcell, hi (μ.mem_col_iff'.mp (μ.nw_of h' (le_refl _) hcell)))
+
+-- presumably easier because they only involve finitely-many values of j'
+instance young_diagram.dec_cell_left (μ : young_diagram)
+  (i j : ℕ) : decidable (∀ {j'}, j' < j → (i, j') ∈ μ) := by apply_instance
+instance young_diagram.dec_cell_up (μ : young_diagram)
+  (i j : ℕ) : decidable (∀ {i'}, i' < i → (i', j) ∈ μ) := by apply_instance
+
 
 def young_diagram.inner_corner.del {μ : young_diagram} (c : μ.inner_corner) : 
 young_diagram :=
-{ cells := finset.erase μ.cells (c.i, c.j),
+{ cells := μ.cells.erase (c.i, c.j), -- finset.erase
   nw_of' := λ i1 i2 j1 j2 hi hj hcell, begin
     rw finset.mem_erase at *,
     split,
-    intro h, rw prod.mk.inj_iff at h, cases h, subst i1, subst j1,
+    intro h, cases h, clear h,
     cases lt_or_eq_of_le hi,
-      exact c.col_down h (μ.nw_of (le_refl _) hj hcell.2),
+      exact c.cell_down h (μ.nw_of (le_refl _) hj hcell.2),
     cases lt_or_eq_of_le hj,
-      exact c.row_right h_1 (μ.nw_of hi (le_refl _) hcell.2),
+      exact c.cell_right h_1 (μ.nw_of hi (le_refl _) hcell.2),
     apply hcell.1, subst i2, subst j2,
     exact μ.nw_of hi hj hcell.2,
   end
 }
 
-def young_diagram.outer_corner.out {μ : young_diagram} (c : μ.outer_corner) : 
+lemma young_diagram.inner_corner.del_def 
+  {μ : young_diagram} (c : μ.inner_corner) : 
+c.del.cells = μ.cells.erase (c.i, c.j) := rfl
+
+@[simp] lemma young_diagram.inner_corner.mem_del
+  {μ : young_diagram} (c : μ.inner_corner) {i j : ℕ} : 
+(i, j) ∈ c.del ↔ (i, j) ≠ (c.i, c.j) ∧ (i, j) ∈ μ := finset.mem_erase
+
+def young_diagram.outer_corner.add {μ : young_diagram} (c : μ.outer_corner) : 
 young_diagram :=
 { cells := insert (c.i, c.j) μ.cells,
   nw_of' := λ i1 i2 j1 j2 hi hj hcell, begin
     rw finset.mem_insert at *,
     cases hcell,
-    rw prod.mk.inj_iff at hcell, cases hcell, subst i2, subst j2,
+    cases hcell,
     cases lt_or_eq_of_le hi,
-      right, exact μ.nw_of (le_refl _) hj (c.col_up h),
+      right, exact μ.nw_of (le_refl _) hj (c.cell_up h),
     cases lt_or_eq_of_le hj,
-      right, exact μ.nw_of hi (le_refl _) (c.row_left h_1),
+      right, exact μ.nw_of hi (le_refl _) (c.cell_left h_1),
     left, subst i1, subst j1,
     exact or.inr (μ.nw_of hi hj hcell),
+  end
+}
+
+lemma young_diagram.outer_corner.add_def
+  {μ : young_diagram} (c : μ.outer_corner) : 
+c.add.cells = insert (c.i, c.j) μ.cells := rfl
+
+@[simp] lemma young_diagram.outer_corner.mem_add
+  {μ : young_diagram} (c : μ.outer_corner) {i j : ℕ} : 
+(i, j) ∈ c.add ↔ (i, j) = (c.i, c.j) ∨ (i, j) ∈ μ := finset.mem_insert
+
+def young_diagram.inner_corner.to_outer
+  {μ : young_diagram} (c : μ.inner_corner) : c.del.outer_corner :=
+{ i := c.i,
+  j := c.j,
+  not_cell := begin 
+    rw young_diagram.inner_corner.mem_del,
+    rw not_and', push_neg, exact λ _, rfl,
+  end,
+  cell_left := λ j' hj, begin
+    rw young_diagram.inner_corner.mem_del,
+    split, exact λ h, ne_of_lt hj (prod.ext_iff.mp h).2,
+    exact μ.nw_of (le_refl _) (le_of_lt hj) c.cell,
+  end,
+  cell_up := λ i' hi, begin
+    rw young_diagram.inner_corner.mem_del,
+    split, exact λ h, ne_of_lt hi (prod.ext_iff.mp h).1,
+    exact μ.nw_of (le_of_lt hi) (le_refl _) c.cell,
   end,
 }
 
+def young_diagram.outer_corner.to_inner 
+  {μ : young_diagram} (c : μ.outer_corner) : c.add.inner_corner :=
+{ i := c.i,
+  j := c.j,
+  cell := begin
+    rw young_diagram.outer_corner.mem_add,
+    left, refl,
+  end,
+  cell_right := λ j' hj, begin
+    rw young_diagram.outer_corner.mem_add, intro h,
+    cases h, exact (ne_of_lt hj).symm (prod.ext_iff.mp h).2,
+    exact c.not_cell (μ.nw_of (le_refl _) (le_of_lt hj) h),
+  end,
+  cell_down := λ i' hi, begin
+    rw young_diagram.outer_corner.mem_add, intro h,
+    cases h, exact (ne_of_lt hi).symm (prod.ext_iff.mp h).1,
+    exact c.not_cell (μ.nw_of (le_of_lt hi) (le_refl _) h),
+  end,
+}
+
+@[simp] lemma young_diagram.outer_inner {μ : young_diagram} (c : μ.inner_corner) :
+  c.to_outer.add = μ :=
+begin
+  ext ⟨i, j⟩,
+  rw [c.to_outer.add.mem_cells, μ.mem_cells, c.to_outer.mem_add, c.mem_del],
+  change (i, j) = (c.i, c.j) ∨ _ ↔ _,
+  by_cases (i, j) = (c.i, c.j),
+    rw [h, eq_self_iff_true, true_or, true_iff],
+    exact c.cell,
+  rw [or_iff_right h, and_iff_right h],
+end
+
+@[simp] lemma young_diagram.inner_outer {μ : young_diagram} (c : μ.outer_corner) :
+  c.to_inner.del = μ :=
+begin
+  ext ⟨i, j⟩,
+  rw [c.to_inner.del.mem_cells, μ.mem_cells, c.to_inner.mem_del, c.mem_add],
+  change (i, j) ≠ (c.i, c.j) ∧ _ ↔ _,
+  by_cases (i, j) = (c.i, c.j),
+    rw [h, ← (false_iff _).mpr c.not_cell, iff_false],
+    push_neg, exact λ h, false.rec _ (h rfl),
+  rw [and_iff_right h, or_iff_right h],
+end
+
 end corners
+
+section examples
 
 @[simp]
 def μ5331 : young_diagram := 
   young_diagram.of_row_lens [5, 3, 3, 1] (by {unfold list_decr, dec_trivial})
 
+def μ5331.corner2 : μ5331.inner_corner :=
+{ i := 2,
+  j := 2,
+  cell := dec_trivial,
+  cell_right := 
+  -- begin
+  --   have : (2 : ℕ).succ < μ5331.row_len 2,
+  --     rw young_diagram.row_len_eq_card,
+  --     -- dec_trivial,
+  --     sorry,
+  --   sorry,
+  -- end,
+  λ j', begin
+    contrapose!, dsimp, rw young_diagram.of_row_lens.mem,
+    exact λ h, nat.lt_succ_iff.mp h,
+  end,
+  cell_down := λ i', begin
+    dsimp, rw [young_diagram.of_row_lens.mem, list.inth],
+    contrapose!, intro h,
 
+    -- beginning of μ
+    repeat { cases i', dec_trivial, simp only [list.nth] at h, },
+    -- rest of μ
+    exfalso, apply not_le_of_lt h, clear h,
+    repeat { cases i', dec_trivial, simp only [list.nth], },
+    -- empty list
+    exact nat.zero_le _,
+  end, }
+
+def μ5331.corner3 : μ5331.outer_corner :=
+{ i := 1,
+  j := 3,
+  not_cell := dec_trivial,
+  cell_left := dec_trivial,
+  -- λ j', begin
+  --   contrapose!, dsimp, rw young_diagram.of_row_lens.mem,
+  --   push_neg, exact id,
+  -- end,
+  cell_up := dec_trivial,
+  -- λ i', begin
+  --   dsimp, rw [young_diagram.of_row_lens.mem, list.inth],
+  --   intro h, rw nat.lt_succ_iff at h,
+  --   -- beginning of μ
+  --   repeat { cases i', dec_trivial, 
+  --            simp only [list.nth], 
+  --            repeat { rw nat.succ_le_succ_iff at h },},
+  --   -- empty list
+  --   exfalso, apply nat.not_succ_le_zero _ h,
+  -- end,
+}
+
+#eval μ5331
+
+#eval μ5331.corner2.del
+
+#eval μ5331.corner3.add
+
+end examples
 
 end young_diagram
